src/hls/GiblePargenproofCommon.v
@@ -1,0 +1,264 @@
+(*
+ * Vericert: Verified high-level synthesis.
+ * Copyright (C) 2023 Yann Herklotz <git@yannherklotz.com>
+ *
+ * This program is free software: you can redistribute it and/or modify
+ * it under the terms of the GNU General Public License as published by
+ * the Free Software Foundation, either version 3 of the License, or
+ * (at your option) any later version.
+ *
+ * This program is distributed in the hope that it will be useful,
+ * but WITHOUT ANY WARRANTY; without even the implied warranty of
+ * MERCHANTABILITY or FITNESS FOR A PARTICULAR PURPOSE.  See the
+ * GNU General Public License for more details.
+ *
+ * You should have received a copy of the GNU General Public License
+ * along with this program.  If not, see <https://www.gnu.org/licenses/>.
+ *)
+
+Require Import compcert.backend.Registers.
+Require Import compcert.common.AST.
+Require Import compcert.common.Errors.
+Require Import compcert.common.Linking.
+Require Import compcert.common.Globalenvs.
+Require Import compcert.common.Memory.
+Require Import compcert.common.Values.
+Require Import compcert.lib.Maps.
+
+Require Import vericert.common.Vericertlib.
+Require Import vericert.hls.GibleSeq.
+Require Import vericert.hls.GiblePar.
+Require Import vericert.hls.Gible.
+Require Import vericert.hls.GiblePargenproofEquiv.
+Require Import vericert.hls.GiblePargen.
+Require Import vericert.hls.Predicate.
+Require Import vericert.hls.Abstr.
+Require Import vericert.hls.AbstrSemIdent.
+Require Import vericert.common.Monad.
+
+Module Import OptionExtra := MonadExtra(Option).
+
+#[local] Open Scope positive.
+#[local] Open Scope forest.
+#[local] Open Scope pred_op.
+
+#[local] Opaque simplify.
+#[local] Opaque deep_simplify.
+
+#[local] Ltac destr := destruct_match; try discriminate; [].
+
+Lemma storev_valid_pointer1 :
+  forall chunk m m' s d b z,
+    Mem.storev chunk m s d = Some m' ->
+    Mem.valid_pointer m b z = true ->
+    Mem.valid_pointer m' b z = true.
+Proof using.
+  intros. unfold Mem.storev in *. destruct_match; try discriminate; subst.
+  apply Mem.valid_pointer_nonempty_perm. apply Mem.valid_pointer_nonempty_perm in H0.
+  eapply Mem.perm_store_1; eauto.
+Qed.
+
+Lemma storev_valid_pointer2 :
+  forall chunk m m' s d b z,
+    Mem.storev chunk m s d = Some m' ->
+    Mem.valid_pointer m' b z = true ->
+    Mem.valid_pointer m b z = true.
+Proof using.
+  intros. unfold Mem.storev in *. destruct_match; try discriminate; subst.
+  apply Mem.valid_pointer_nonempty_perm. apply Mem.valid_pointer_nonempty_perm in H0.
+  eapply Mem.perm_store_2; eauto.
+Qed.
+
+Definition valid_mem m m' :=
+  forall b z, Mem.valid_pointer m b z = Mem.valid_pointer m' b z.
+
+#[global] Program Instance valid_mem_Equivalence : Equivalence valid_mem.
+Next Obligation. unfold valid_mem; auto. Qed. (* Reflexivity *)
+Next Obligation. unfold valid_mem; auto. Qed. (* Symmetry *)
+Next Obligation. unfold valid_mem; eauto. Qed. (* Transitity *)
+
+Lemma storev_valid_pointer :
+  forall chunk m m' s d,
+    Mem.storev chunk m s d = Some m' ->
+    valid_mem m m'.
+Proof using.
+  unfold valid_mem. symmetry.
+  intros. destruct (Mem.valid_pointer m b z) eqn:?;
+                   eauto using storev_valid_pointer1.
+  apply not_true_iff_false.
+  apply not_true_iff_false in Heqb0.
+  eauto using storev_valid_pointer2.
+Qed.
+
+Lemma storev_cmpu_bool :
+  forall m m' c v v0,
+    valid_mem m m' ->
+    Val.cmpu_bool (Mem.valid_pointer m) c v v0 = Val.cmpu_bool (Mem.valid_pointer m') c v v0.
+Proof using.
+  unfold valid_mem.
+  intros. destruct v, v0; crush.
+  { destruct_match; crush.
+    destruct_match; crush.
+    destruct_match; crush.
+    apply orb_true_iff in H1.
+    inv H1. rewrite H in H2. rewrite H2 in Heqb1.
+    simplify. rewrite H0 in Heqb1. crush.
+    rewrite H in H2. rewrite H2 in Heqb1.
+    rewrite H0 in Heqb1. crush.
+    destruct_match; auto. simplify.
+    apply orb_true_iff in H1.
+    inv H1. rewrite <- H in H2. rewrite H2 in Heqb1.
+    simplify. rewrite H0 in Heqb1. crush.
+    rewrite <- H in H2. rewrite H2 in Heqb1.
+    rewrite H0 in Heqb1. crush. }
+
+  { destruct_match; crush.
+    destruct_match; crush.
+    destruct_match; crush.
+    apply orb_true_iff in H1.
+    inv H1. rewrite H in H2. rewrite H2 in Heqb1.
+    simplify. rewrite H0 in Heqb1. crush.
+    rewrite H in H2. rewrite H2 in Heqb1.
+    rewrite H0 in Heqb1. crush.
+    destruct_match; auto. simplify.
+    apply orb_true_iff in H1.
+    inv H1. rewrite <- H in H2. rewrite H2 in Heqb1.
+    simplify. rewrite H0 in Heqb1. crush.
+    rewrite <- H in H2. rewrite H2 in Heqb1.
+    rewrite H0 in Heqb1. crush. }
+
+  { destruct_match; auto. destruct_match; auto; crush.
+    { destruct_match; crush.
+      { destruct_match; crush.
+        setoid_rewrite H in H0; eauto.
+        setoid_rewrite H in H1; eauto.
+        rewrite H0 in Heqb. rewrite H1 in Heqb; crush.
+      }
+      { destruct_match; crush.
+        setoid_rewrite H in Heqb0; eauto.
+        rewrite H0 in Heqb0. rewrite H1 in Heqb0; crush. } }
+    { destruct_match; crush.
+      { destruct_match; crush.
+        setoid_rewrite H in H0; eauto.
+        setoid_rewrite H in H1; eauto.
+        rewrite H0 in Heqb0. rewrite H1 in Heqb0; crush.
+      }
+      { destruct_match; crush.
+        setoid_rewrite H in Heqb0; eauto.
+        rewrite H0 in Heqb0. rewrite H1 in Heqb0; crush. } } }
+Qed.
+
+Lemma storev_eval_condition :
+  forall m m' c rs,
+    valid_mem m m' ->
+    Op.eval_condition c rs m = Op.eval_condition c rs m'.
+Proof using.
+  intros. destruct c; crush.
+  destruct rs; crush.
+  destruct rs; crush.
+  destruct rs; crush.
+  eapply storev_cmpu_bool; eauto.
+  destruct rs; crush.
+  destruct rs; crush.
+  eapply storev_cmpu_bool; eauto.
+Qed.
+
+Lemma eval_operation_valid_pointer :
+  forall A B (ge: Genv.t A B) sp op args m m' v,
+    valid_mem m m' ->
+    Op.eval_operation ge sp op args m' = Some v ->
+    Op.eval_operation ge sp op args m = Some v.
+Proof.
+  intros * VALID OP. destruct op; auto.
+  - destruct cond; auto; cbn in *.
+    + repeat destruct_match; auto. setoid_rewrite <- storev_cmpu_bool in OP; eauto.
+    + repeat destruct_match; auto. setoid_rewrite <- storev_cmpu_bool in OP; eauto.
+  - destruct c; auto; cbn in *.
+    + repeat destruct_match; auto. setoid_rewrite <- storev_cmpu_bool in OP; eauto.
+    + repeat destruct_match; auto. setoid_rewrite <- storev_cmpu_bool in OP; eauto.
+Qed.
+
+Lemma bb_memory_consistency_eval_operation :
+  forall A B (ge: Genv.t A B) sp state i state' args op v,
+    step_instr ge sp (Iexec state) i (Iexec state') ->
+    Op.eval_operation ge sp op args (is_mem state) = Some v ->
+    Op.eval_operation ge sp op args (is_mem state') = Some v.
+Proof.
+  inversion_clear 1; intro EVAL; auto.
+  cbn in *.
+  eapply eval_operation_valid_pointer. unfold valid_mem. symmetry.
+  eapply storev_valid_pointer; eauto.
+  auto.
+Qed.
+
+Lemma truthy_dflt :
+  forall ps p,
+    truthy ps p -> eval_predf ps (dfltp p) = true.
+Proof. intros. destruct p; cbn; inv H; auto. Qed.
+
+Lemma exists_sem_pred :
+  forall A B C (ctx: @ctx A) s pr r v,
+    @sem_pred_expr A B C pr s ctx r v ->
+    exists r',
+      NE.In r' r /\ s ctx (snd r') v.
+Proof.
+  induction r; crush.
+  - inv H. econstructor. split. constructor. auto.
+  - inv H.
+    + econstructor. split. constructor. left; auto. auto.
+    + exploit IHr; eauto. intros HH. inversion_clear HH as [x HH']. inv HH'.
+      econstructor. split. constructor. right. eauto. auto.
+Qed.
+
+Definition predicated_not_inP {A} (p: Gible.predicate) (l: predicated A) :=
+  forall op e, NE.In (op, e) l -> ~ PredIn p op.
+
+Lemma predicated_not_inP_cons :
+  forall A p (a: (pred_op * A)) l,
+    predicated_not_inP p (NE.cons a l) ->
+    predicated_not_inP p l.
+Proof.
+  unfold predicated_not_inP; intros. eapply H. econstructor. right; eauto.
+Qed.
+
+Lemma match_states_list :
+  forall A (rs: Regmap.t A) rs',
+  (forall r, rs !! r = rs' !! r) ->
+  forall l, rs ## l = rs' ## l.
+Proof. induction l; crush. Qed.
+
+Lemma PTree_matches :
+  forall A (v: A) res rs rs',
+  (forall r, rs !! r = rs' !! r) ->
+  forall x, (Regmap.set res v rs) !! x = (Regmap.set res v rs') !! x.
+Proof.
+  intros; destruct (Pos.eq_dec x res); subst;
+  [ repeat rewrite Regmap.gss by auto
+  | repeat rewrite Regmap.gso by auto ]; auto.
+Qed.
+
+Lemma truthy_dec:
+  forall ps a, truthy ps a \/ falsy ps a.
+Proof.
+  destruct a; try case_eq (eval_predf ps p); intuition (constructor; auto).
+Qed.
+
+Lemma truthy_match_state :
+  forall ps ps' p,
+    (forall x, ps !! x = ps' !! x) ->
+    truthy ps p ->
+    truthy ps' p.
+Proof.
+  intros; destruct p; inv H0; constructor; auto.
+  erewrite eval_predf_pr_equiv; eauto.
+Qed.
+
+Lemma falsy_match_state :
+  forall ps ps' p,
+    (forall x, ps !! x = ps' !! x) ->
+    falsy ps p ->
+    falsy ps' p.
+Proof.
+  intros; destruct p; inv H0; constructor; auto.
+  erewrite eval_predf_pr_equiv; eauto.
+Qed.
